\documentclass[exercise]{math-standalone}

\begin{document}
\begin{exercise}{
    Számítsuk ki az alábbi skalármezők gradiensét! Hattassuk a függvényekre
    a Laplace-operátort is!
  }
  \begin{multicols}{2}
    \begin{enumerate}[a)]
      \item $f(\rvec r) = xyz$
      \item $g(\rvec r) = 6x^y + \sin e^z$
      \item $h(\rvec r) = \rvec r^2 / 2$
      \item $i(\rvec r) = xy + xz + yz$
      \item $j(\rvec r) = 2 x^2 y + x z^2 + 6 y$
    \end{enumerate}
  \end{multicols}

  \exsol{%
    \begin{enumerate}[a)]
      \item $f(\rvec r) = xyz$
            \[
              \grad f
              =
              \nabla f
              =
              \left(
              \pdv{f}{x}; \pdv{f}{y}; \pdv{f}{z}
              \right)^\transpose
              =
              \begin{bmatrix}
                yz \\ xz \\ xy
              \end{bmatrix}
            \]
            \[
              \laplacian f
              =
              \Div \grad f
              =
              \pdv{yz}{x} + \pdv{xz}{y} + \pdv{xy}{z}
              =
              0
            \]

      \item $g(\rvec r) = 6x^y + \sin e^z$
            \[
              \grad g
              =
              \nabla g
              =
              \left(
              \pdv{g}{x}; \pdv{g}{y}; \pdv{g}{z}
              \right)^\transpose
              = \begin{bmatrix}
                6 y x^{y - 1} \\
                6 x^y \ln x   \\
                e^z \cos e^z
              \end{bmatrix}
            \]
            \begin{align*}
              \laplacian g
               & =
              \Div \grad g
              =
              \pdv{6 y x^{y - 1}}{x} +
              \pdv{6 x^y \ln x}{y} +
              \pdv{e^z \cos e^z}{z}
              \\
               & =
              6 y (y - 1) x^{y - 2} + 6 x^y \ln^2 x + e^z \cos e^z - e^{2z} \sin e^z
            \end{align*}

      \item $h(\rvec r) = \rvec r^2 / 2 = (x^2 + y^2 + z^2) / 2$
            \[
              \grad h
              =
              \nabla h
              =
              \left(
              \pdv{h}{x}; \pdv{h}{y}; \pdv{h}{z}
              \right)
              =
              \begin{bmatrix}
                x \\ y \\ z
              \end{bmatrix}
              =
              \rvec r
            \]
            \[
              \laplacian h
              =
              \Div \grad h
              =
              \pdv{x}{x} + \pdv{y}{y} + \pdv{z}{z}
              =
              3
            \]

      \item $i(\rvec r) = xy + xz + yz$
            \[
              \grad i
              =
              \nabla i
              =
              \left(
              \pdv{i}{x}; \pdv{i}{y}; \pdv{i}{z}
              \right)
              =
              \begin{bmatrix}
                y + z \\ x + z \\ x + y
              \end{bmatrix}
            \]
            \[
              \laplacian i
              =
              \Div \grad i
              =
              \pdv{(y + z)}{x} + \pdv{(x + z)}{y} + \pdv{(x + y)}{z}
              =
              0
            \]

      \item $j(\rvec r) = 2 x^2 y + x z^2 + 6 y$
            \[
              \grad j
              =
              \nabla j
              =
              \left(
              \pdv{j}{x}; \pdv{j}{y}; \pdv{j}{z}
              \right)
              =
              \begin{bmatrix}
                4 x y + z^2 \\
                2 x^2 + 6   \\
                2 x z
              \end{bmatrix}
            \]
            \[
              \laplacian j
              =
              \Div \grad j
              =
              \pdv{4 x y + z^2}{x} + \pdv{2 x^2 + 6}{y} + \pdv{2 x z}{z}
              =
              4 y + 2 x
            \]
    \end{enumerate}
  }
\end{exercise}
\end{document}
